\documentclass[12pt]{article}
\usepackage{graphicx}
\usepackage{xspace}
\usepackage{color, colortbl}
\usepackage{amssymb}
\pagestyle{empty}
\definecolor{Gray}{gray}{0.9}
\textwidth      165mm
\textheight     240mm
\topmargin      -18mm
\oddsidemargin  -2mm
\evensidemargin 2mm
\newcommand{\impl}{\mathbin{\Rightarrow}}
\newcommand{\biim}{\mathbin{\Leftrightarrow}}
\renewcommand{\theenumi}{\alph{enumi}}

\author{Emmanuel Macario - 831659}
\title{COMP30026 Models of Computation Assignment 1}
\date{September, 2018}

\begin{document}

\maketitle

\subsection*{Challenge 1}
\begin{enumerate}
\item 
$\begin{array}{|ccc|c|c|}
   \hline
   P & Q & R & ((\neg P \land Q) \impl \neg R) \impl R & R
\\ \hline
    0 & 0 & 0 & 0 & 0
\\ 0 & 0 & 1 & 1 & 1
\\ 0 & 1 & 0 & 0 & 0
\\ 0 & 1 & 1 & 1 & 1
\\ 1 & 0 & 0 & 0 & 0
\\ 1 & 0 & 1 & 1 & 1
\\ 1 & 1 & 0 & 0 & 0
\\ 1 & 1 & 1 & 1 & 1
\\ \hline
\end{array}$
$\therefore ((\neg P \land Q) \impl \neg R) \impl R \equiv R$
\bigskip

\item 
$\begin{array}{|ccc|c|c|}
   \hline
   P & Q & R & (P \impl (Q \lor R)) \land (P \biim Q) & P \biim Q
\\ \hline
    0 & 0 & 0 & 1 & 1
\\ 0 & 0 & 1 & 1 & 1
\\ 0 & 1 & 0 & 0 & 0
\\ 0 & 1 & 1 & 0 & 0
\\ 1 & 0 & 0 & 0 & 0
\\ 1 & 0 & 1 & 0 & 0
\\ 1 & 1 & 0 & 1 & 1
\\ 1 & 1 & 1 & 1 & 1
\\ \hline
\end{array}$
$\therefore (P \impl (Q \lor R)) \land (P \biim Q) \equiv P \biim Q$
\bigskip

\item
$\begin{array}{|cc|c|c|}
   \hline
   P & Q & P \impl (P \biim Q) & P \impl Q
\\ \hline
    0 & 0 & 1 & 1
\\ 0 & 1 & 1 & 1
\\ 1 & 0 & 0 & 0
\\ 1 & 1 & 1 & 1
\\ \hline
\end{array}$
$\therefore P \impl (P \biim Q) \equiv P \impl Q$
\bigskip

\item
$\begin{array}{|ccc|c|c|}
   \hline
   P & Q & R & P \lor (R \impl Q) & (Q \impl P) \impl (R \impl P)
\\ \hline
    0 & 0 & 0 & 1 & 1
\\ 0 & 0 & 1 & 0 & 0
\\ 0 & 1 & 0 & 1 & 1
\\ 0 & 1 & 1 & 1 & 1
\\ 1 & 0 & 0 & 1 & 1
\\ 1 & 0 & 1 & 1 & 1
\\ 1 & 1 & 0 & 1 & 1
\\ 1 & 1 & 1 & 1 & 1
\\ \hline
\end{array}$
$\therefore P \lor (R \impl Q) \equiv (Q \impl P) \impl (R \impl P)$
\bigskip

\end{enumerate}


\subsection*{Challenge 2}

Firstly, let us define both inhabitant's statements in propositional logic.
Inhabitant $P$'s statements are equivalent to $\neg Q$ and $Q'$, respectively. 
Inhabitant $Q$'s statements are equivalent to $P$ and $\neg P'$, respectively.

\bigskip
\noindent
We are given information that the statements given by the inhabitants $P$ and $Q$ 
respectively must be either true or false, but \emph{cannot} be a mixture of both. 
In other words, if an inhabitant lies, then every statement they say is guaranteed to 
be a false statement.

\bigskip
\noindent
This means that if inhabitant $P$ is telling the truth, then $\neg Q \land Q'$ is true, 
otherwise $Q \land \neg Q'$ must be true. Similarly, if inhabitant $Q$ is telling the truth,
then $P \land \neg P'$ must be true, otherwise $\neg P \land P'$ must be true.


\bigskip
\noindent
Let $A$ mean $P$ \emph{is telling the truth}, and $B$ mean $Q$ is \emph{telling
the truth}. We can surmise when $P$ and $Q$ are lying or telling the truth via truth tables.

\bigskip
\begin{minipage}{0.5\textwidth}
\begin{center}
$\begin{array}{|cc|c|}
   \hline
   P & P' & A
\\ \hline
   0 & 0 & 1
\\ 0 & 1 & 0
\\ 1 & 0 & 0
\\ 1 & 1 & 1
\\ \hline
\end{array}$
\end{center}
\end{minipage}
\begin{minipage}{0.35\textwidth}
\begin{center}
$\begin{array}{|cc|c|}
   \hline
   Q & Q' & B
\\ \hline
   0 & 0 & 1
\\ 0 & 1 & 0
\\ 1 & 0 & 0
\\ 1 & 1 & 1
\\ \hline
\end{array}$
\end{center}
\end{minipage}

\bigskip
\noindent
It can be seen that $P$ is truthful when $P \biim P'$ is true, and lies when $P 
\oplus P'$ is true. The same notions hold for inhabitant $Q$, with respect to 
literals $Q$ and $Q'$.

\bigskip
\noindent
Using the formulas generated above, we can now extract the maximal amount of information 
provided by the two  inhabitants, in the form of propositional formulas (1) and (2), both of which
must be true.

\medskip
\begin{equation}
((P \biim P') \land (\neg Q \land Q')) \oplus ((P \oplus P') \land (Q \land \neg Q'))
\end{equation}
\begin{equation}
((Q \biim Q') \land (P \land \neg P')) \oplus ((Q \oplus Q') \land (\neg P \land P'))
\end{equation}

\bigskip
\noindent
Using a truth table, we can determine for each of $P$ and $Q$ whether they 
are a knight or a knave, and whether they are healthy or sick.

\bigskip
\begin{center}
\resizebox{0.95\textwidth}{!}{$\begin{array}{|cccc|c|c|}
   \hline
   P & P' & Q & Q' & ((P \biim P') \land (\neg Q \land Q')) \oplus ((P \oplus P') \land (Q \land \neg Q')) & 
   ((Q \biim Q') \land (P \land \neg P')) \oplus ((Q \oplus Q') \land (\neg P \land P'))
\\ \hline
   0 & 0 & 0 & 0 & 0 & 0 
\\ 0 & 0 & 0 & 1 & 1 & 0
\\ 0 & 0 & 1 & 0 & 0 & 0
\\ 0 & 0 & 1 & 1 & 0 & 0 
\\ 0 & 1 & 0 & 0 & 0 & 0 
\\ 0 & 1 & 0 & 1 & 0 & 1 
\\ \rowcolor{Gray}
   0 & 1 & 1 & 0 & 1 & 1 
\\ 0 & 1 & 1 & 1 & 0 & 0
\\ 1 & 0 & 0 & 0 & 0 & 1 
\\ 1 & 0 & 0 & 1 & 0 & 0 
\\ 1 & 0 & 1 & 0 & 1 & 0 
\\ 1 & 0 & 1 & 1 & 0 & 1 
\\ 1 & 1 & 0 & 0 & 0 & 0 
\\ 1 & 1 & 0 & 1 & 1 & 0 
\\ 1 & 1 & 1 & 0 & 0 & 0 
\\ 1 & 1 & 1 & 1 & 0 & 0
\\ \hline
\end{array}$}
\end{center}

\bigskip
\noindent
We know that both formulas must be true. Therefore,
there is only \emph{one} possible scenario. That is, $P$
is a \emph{healthy knave} and $Q$ is a \emph{sick knight}.

% CHALLENGE 3
\subsection*{Challenge 3}
\begin{enumerate}
  \item
Consider the interpretation $I$ with domain $D$ = \{0,1\} and $P(0)$. Additionally, 
let $Q$ always be \emph{false}.

\bigskip
\noindent
For this interpretation, it can be seen that $I \vDash \forall x
(P(x)) \impl Q$, but $I \nvDash \forall x(P(x) \impl Q)$.
Hence, $\forall x(P(x)) \impl Q \nvDash \forall x(P(x) \impl Q)$.

\bigskip
\noindent
Therefore, $\forall x (P(x)) \impl Q$ is \emph{not} equivalent to
$\forall x(P(x) \impl Q)$.

\item
\end{enumerate}


% CHALLENGE 4
\subsection*{Challenge 4}
\begin{enumerate}
  \item $\forall x \forall y(M(x,y) \impl F(x))$
  \item $\forall x \forall y((U(x) \land M(y,x)) \impl U(y))$
  \item $\forall x((F(x) \land U(x) \land B(x)) \impl D(x))$
  \item $\forall x \forall y((U(x) \land M(x,y) \land D(x)) \impl D(y))$
  \item $\forall x((S(x) \land U(x)) \impl B(x))$
\end{enumerate}

\bigskip
\noindent
The \emph{Horn clauses} generated are as follows:
\begin{enumerate}
  \item $\{\neg M(x,y), F(x)\}$
  \item $\{\neg U(x), \neg M(y,x), U(y)\}$
  \item $\{\neg F(x), \neg U(x), \neg B(x), D(x)\}$
  \item $\{\neg U(x), \neg M(x), \neg D(x), D(y)\}$
  \item $\{\neg S(x), \neg U(x), B(x)\}$
\end{enumerate}

\bigskip
\noindent
Now, we must express statement (f) in first-order predicate logic.

\bigskip
f.  $\forall x \forall y((U(x) \land M(y,x) \land S(y)) \impl D(x))$

\bigskip
\noindent
The negation of (f) in clausal form is: 

$\neg \forall x \forall y((U(x) \land M(y,x) \land S(y)) \impl D(x))$

$\rightsquigarrow \exists x \neg \forall y((U(x) \land M(y,x) \land S(y)) \impl D(x))$

$\rightsquigarrow \exists x \exists y(U(x) \land M(y,x) \land S(y) \land \neg D(x))$

$\rightsquigarrow \exists y(U(a) \land M(y,a) \land S(y) \land \neg D(a))$

$\rightsquigarrow (U(a) \land M(b,a) \land S(b) \land \neg D(a))$

\bigskip
\noindent
Which produces \emph{four} clauses: 

$\{U(a)\}, \{M(b,a)\}, \{S(b)\}, \{\neg D(a)\}$

\bigskip
\noindent
Now, we can find a refutation of the set of nine clauses.


\bigskip
\noindent
By the refutation proof shown above, we have proven that the conjunction of
premise statements (a)-(e) and the negation of conclusion statement (f) is
unsatisfiable. 

\bigskip
\noindent
$\therefore$ (f) is a logical consequence of statements (a)-(e)



% CHALLENGE 5
\subsection*{Challenge 5}

\begin{enumerate}
  \item (a1) $\forall x \forall y(N(x,y) \impl N(y,x))\\\\$
        (a2) $\forall x \forall y \exists u((M(u,x) \land \neg M(u,y)) \impl N(x,y))\\\\$
        (a3) $\forall x(\neg \exists u(M(u,x)) \impl E(x))\\\\$
        (a4) $\forall x \forall y \forall u((D(x,y) \land M(u,x)) \impl \neg M(u,y))$
\end{enumerate}


% CHALLENGE 6
\subsection*{Challenge 6}
See Grok.


\end{document}